bedrock2/src/FlattenExpr.v
@@ -7,10 +7,13 @@ Require Import compiler.NameGen.
 Require Import bbv.DepEqNat.
 Require Import compiler.NameWithEq.
 Require Import riscv.util.BitWidths.
+Require Import riscv.Utility.
+
 
 Section FlattenExpr.
 
-  Context {Bw: BitWidths}.
+  Context {mword: Set}.
+  Context {MW: MachineWidth mword}.
 
   Context {Name: NameWithEq}.
   Context {FName: NameWithEq}.
@@ -19,24 +22,24 @@ Section FlattenExpr.
 
   Existing Instance eq_name_dec.
 
-  Context {stateMap: MapFunctions var (word wXLEN)}.
-  Notation state := (map var (word wXLEN)).
+  Context {stateMap: MapFunctions var mword}.
+  Notation state := (map var mword).
   Context {varset: SetFunctions var}.
   Notation vars := (set var).
 
   Context {NGstate: Type}.
   Context {NG: NameGen var NGstate}.
 
-  Context {funcMap: MapFunctions func (list var * list var * @FlatImp.stmt Bw Name FName)}.
-  Notation env := (map func (list var * list var * @FlatImp.stmt Bw Name FName)).
+  Context {funcMap: MapFunctions func (list var * list var * @FlatImp.stmt mword Name FName)}.
+  Notation env := (map func (list var * list var * @FlatImp.stmt mword Name FName)).
 
-  Ltac state_calc := state_calc_generic (@name Name) (word wXLEN).
+  Ltac state_calc := state_calc_generic (@name Name) mword.
   Ltac set_solver := set_solver_generic (@name Name).
 
   (* returns stmt and var into which result is saved, and new fresh name generator state
      TODO use state monad? *)
-  Fixpoint flattenExpr(ngs: NGstate)(e: @ExprImp.expr Bw Name):
-    (@FlatImp.stmt Bw Name FName  * var * NGstate) :=
+  Fixpoint flattenExpr(ngs: NGstate)(e: @ExprImp.expr mword Name):
+    (@FlatImp.stmt mword Name FName  * var * NGstate) :=
     match e with
     | ExprImp.ELit n =>
         let '(x, ngs') := genFresh ngs in
@@ -53,8 +56,9 @@ Section FlattenExpr.
         (FlatImp.SSeq s1 (FlatImp.SSeq s2 (FlatImp.SOp x op r1 r2)), x, ngs''')
     end.
 
-  Definition flattenCall(ngs: NGstate)(binds: list var)(f: func)(args: list (@ExprImp.expr Bw Name)):
-    @FlatImp.stmt Bw Name FName * NGstate :=
+  Definition flattenCall(ngs: NGstate)(binds: list var)(f: func)
+             (args: list (@ExprImp.expr mword Name)):
+    @FlatImp.stmt mword Name FName * NGstate :=
     let '(compute_args, argvars, ngs) :=
           List.fold_right
             (fun e '(c, vs, ngs) =>
@@ -65,7 +69,7 @@ Section FlattenExpr.
       (FlatImp.SSeq compute_args (FlatImp.SCall binds f argvars), ngs).
 
   (* returns statement and new fresh name generator state *)
-  Fixpoint flattenStmt(ngs: NGstate)(s: @ExprImp.stmt Bw Name FName): (@FlatImp.stmt Bw Name FName * NGstate) :=
+  Fixpoint flattenStmt(ngs: NGstate)(s: @ExprImp.stmt mword Name FName): (@FlatImp.stmt mword Name FName * NGstate) :=
     match s with
     | ExprImp.SLoad x a =>
         let '(s, r, ngs') := flattenExpr ngs a in
@@ -124,9 +128,9 @@ Section FlattenExpr.
       specialize (IHargs binds ngs).
       rewrite E0 in IHargs.
       specialize IHargs with (1 := eq_refl).
-      unfold FlatImp.stmt_size. fold (@FlatImp.stmt_size Bw Name FName).
+      unfold FlatImp.stmt_size. fold (@FlatImp.stmt_size mword Name FName).
       unfold ExprImp.stmt_size.
-      unfold FlatImp.stmt_size in IHargs; fold (@FlatImp.stmt_size Bw Name FName) in IHargs.
+      unfold FlatImp.stmt_size in IHargs; fold (@FlatImp.stmt_size mword Name FName) in IHargs.
       unfold ExprImp.stmt_size in IHargs.
       rewrite map_cons. rewrite fold_right_cons.
       destruct p.
@@ -271,7 +275,7 @@ Section FlattenExpr.
      "only_differ initialL (vars_range firstFree (S resVar)) finalL"
      this needn't be part of this lemma, because it follows from
      flattenExpr_modVars_spec and FlatImp.modVarsSound *)
-  Lemma flattenExpr_correct_aux env : forall e ngs1 ngs2 resVar (s: @FlatImp.stmt Bw Name FName) initialH initialL initialM res,
+  Lemma flattenExpr_correct_aux env : forall e ngs1 ngs2 resVar (s: @FlatImp.stmt mword Name FName) initialH initialL initialM res,
     flattenExpr ngs1 e = (s, resVar, ngs2) ->
     extends initialL initialH ->
     undef initialH (allFreshVars ngs1) ->
@@ -310,21 +314,28 @@ Section FlattenExpr.
       destruct IHe2 as [fuel2 [preFinalL [Ev2 G2]]].
       remember (Datatypes.S (Datatypes.S (fuel1 + fuel2))) as f0.
       remember (Datatypes.S (fuel1 + fuel2)) as f.
-      exists (Datatypes.S f0) (put preFinalL resVar (Op.eval_binop op w w0)).
+      exists (Datatypes.S f0) (put preFinalL resVar (Op.eval_binop op m m0)).
       pose_flatten_var_ineqs.
       split; [|apply get_put_same].
       simpl. fuel_increasing_rewrite.
       subst f0. simpl. fuel_increasing_rewrite.
       subst f. simpl.
       rename n0 into v.
-      assert (get preFinalL v = Some w) as G1'. {
+      assert (get preFinalL v = Some m) as G1'. {
         state_calc.
       }
       rewrite G1'. simpl. rewrite G2. simpl. reflexivity.
   Qed.
 
-  Context {funcMap': MapFunctions func (list var * list var * @ExprImp.stmt Bw Name FName)}.
-  Notation env' := (map func (list var * list var * @ExprImp.stmt Bw Name FName)).
+  Context {funcMap': MapFunctions func (list var * list var * @ExprImp.stmt mword Name FName)}.
+  Notation env' := (map func (list var * list var * @ExprImp.stmt mword Name FName)).
+
+  Ltac simpl_regb_eq :=
+      rewrite? (proj2 (reg_eqb_true _ _) eq_refl);
+      repeat match goal with
+             | H: _ |- _ => rewrite <- reg_eqb_false in H; rewrite H
+             | H: _ |- _ => rewrite <- reg_eqb_true in H; rewrite H
+             end.
 
   Lemma flattenStmt_correct_aux:
     forall fuelH sH sL ngs ngs' initialH finalH initialL initialM finalM,
@@ -434,14 +445,16 @@ Section FlattenExpr.
         simpl in *.
         fuel_increasing_rewrite.
         subst tempFuel.
-        simpl. rewrite G. simpl. simpl_if.
+        simpl. rewrite G. simpl.
+        simpl_regb_eq.
         fuel_increasing_rewrite.
         reflexivity.
     - inversions F. repeat destruct_one_match_hyp. destruct_pair_eqs. subst.
       pose_flatten_var_ineqs.
       rename cond into condH, s into condL, s0 into sL1, s1 into sL2.
       pose proof flattenExpr_correct_aux as P.
-      specialize (P empty_map) with (initialM := initialM) (res := $0) (1 := E) (2 := Ex).
+      specialize (P empty_map) with
+          (initialM := initialM) (res := (@zero mword MW)) (1 := E) (2 := Ex).
       specializes P; [eassumption|eassumption|].
       destruct P as [fuelLcond [initial2L [Evcond G]]].
       pose_flatten_var_ineqs.
@@ -457,7 +470,8 @@ Section FlattenExpr.
         simpl in *.
         fuel_increasing_rewrite.
         subst tempFuel.
-        simpl. rewrite G. simpl. simpl_if.
+        simpl. rewrite G. simpl.
+        simpl_regb_eq.
         fuel_increasing_rewrite.
         reflexivity.
     - simpl in Di.
@@ -489,7 +503,7 @@ Section FlattenExpr.
       refine (conj _ Ex2).
       simpl in *.
       fuel_increasing_rewrite.
-      rewrite G. simpl. simpl_if.
+      rewrite G. simpl. simpl_regb_eq.
       fuel_increasing_rewrite.
       fuel_increasing_rewrite.
       reflexivity.
@@ -498,7 +512,7 @@ Section FlattenExpr.
       simpl in F. do 3 destruct_one_match_hyp. destruct_pair_eqs. subst.
       rename s into sCond, s0 into sBody.
       pose proof (flattenExpr_correct_aux empty_map) as P.
-      specialize P with (res := $0) (initialM := initialM) (1 := E) (2 := Ex).
+      specialize P with (res := (@zero mword MW)) (initialM := initialM) (1 := E) (2 := Ex).
       specializes P; [eassumption|eassumption|].
       destruct P as [fuelLcond [initial2L [EvcondL G]]].
       exists (S fuelLcond) initial2L.
@@ -506,7 +520,7 @@ Section FlattenExpr.
       split; [|state_calc].
       simpl in*.
       fuel_increasing_rewrite.
-      rewrite G. simpl. simpl_if. reflexivity.
+      rewrite G. simpl. simpl_regb_eq. reflexivity.
     - simpl in F. do 2 destruct_one_match_hyp. inversions F.
       pose proof IHfuelH as IHfuelH2.
       specializes IHfuelH.
@@ -534,7 +548,7 @@ Section FlattenExpr.
     - rewrite empty_is_empty in Ev0. inversion Ev0.
   Qed.
 
-  Definition ExprImp2FlatImp(s: @ExprImp.stmt Bw Name FName): @FlatImp.stmt Bw Name FName :=
+  Definition ExprImp2FlatImp(s: @ExprImp.stmt mword Name FName): @FlatImp.stmt mword Name FName :=
     fst (flattenStmt (freshNameGenState (ExprImp.allVars_stmt s)) s).
 
   Lemma flattenStmt_correct: forall fuelH sH sL initialM finalH finalM,
